MyOCL.thy
@@ -45,9 +45,31 @@ COMMENT *)
 (* projVal: given a column-expression and a row --either in person or enrollment table--,
 it returns the corresonding value *)
 
-fun projValAtt :: "att \<Rightarrow> val \<Rightarrow> val" where 
-"projValAtt AGE (VPerson (P page pemail)) = VInt page"
-| "projValAtt EMAIL (VPerson (P page pemail)) = VString pemail"
-| "projValAtt att (VObj var (OM [] es)) = VNULL"
+fun getAgePerson :: "Person \<Rightarrow> nat" where
+"getAgePerson (P age email) = age"
 
+fun getEmailPerson :: "Person \<Rightarrow> string" where
+"getEmailPerson (P age email) = email"
+
+fun projValAtt :: "att \<Rightarrow> val \<Rightarrow> val" where 
+"projValAtt AGE (VPerson p) = VInt (getAgePerson p)"
+| "projValAtt EMAIL (VPerson p) = VString (getEmailPerson p)"
+
+fun getAssociationEnd :: "as \<Rightarrow> Enrollment \<Rightarrow> Person" where
+"getAssociationEnd STUDENTS (E students lecturers) = students"
+  | "getAssociationEnd LECTURERS (E students lecturers) = lecturers"
+
+fun projValAs :: "as \<Rightarrow> val \<Rightarrow> Enrollment list \<Rightarrow> val list" where
+"projValAs LECTURERS (VObj var) [] = []"
+| "projValAs LECTURERS (VObj var) (e#es) = 
+(if (getAssociationEnd STUDENTS e) = (PVObj var)
+then ((VPerson (getAssociationEnd LECTURERS e))#(projValAs LECTURERS (VObj var) es))
+else (projValAs LECTURERS (VObj var) es))"
+(*
+"projValAs LECTURERS (VPerson p) [] = []"
+| "projValAs LECTURERS (VPerson p) (e#es) = 
+(if (getAssociationEnd STUDENTS e) = p 
+then ((VPerson (getAssociationEnd STUDENTS e))#(projValAs LECTURERS (VPerson p) es))
+else (projValAs LECTURERS (VPerson p) es))"
+*)
 end
